proof of concept for opaque specs style on MD5

code/hash-new/Hacl.Hash.Core.MD5.fst
@@ -84,6 +84,11 @@ let t_idx = (n: U32.t { 1 <= U32.v n /\ U32.v n <= 64 } )
 inline_for_extraction
 let (<<<) = Spec.rotl
 
+(*
+ * In each of the stateful functions, to prove their equivalence with the spec functions, call the related reveal lemmas
+ * Also, calling sequence extensional equality explicitly is better and quicker
+ *)
+
 inline_for_extraction
 val round_op_gen
   (f: (U32.t -> U32.t -> U32.t -> Tot U32.t))
@@ -106,8 +111,7 @@ val round_op_gen
     B.as_seq h' abcd == Spec.round_op_gen f (B.as_seq h abcd) (E.seq_uint32_of_le 16 (B.as_seq h x)) (U32.v a) (U32.v b) (U32.v c) (U32.v d) (U32.v k) s (U32.v i)
   ))
 
-#reset-options "--z3rlimit 16" // --using_facts_from '* -FStar.Int8 -FStar.Int16 -FStar.Int32 -FStar.Int64 -FStar.Int128 -FStar.UInt16 -FStar.UInt64 -FStar.UInt128'"
-
+#push-options "--z3rlimit 10"
 let round_op_gen f abcd x a b c d k s i =
   let h = HST.get () in
   assert_norm (64 / 4 == 16);
@@ -122,10 +126,13 @@ let round_op_gen f abcd x a b c d k s i =
   let ti = t (i `U32.sub` 1ul) in
   let v = (vb `U32.add_mod` ((va `U32.add_mod` f vb vc vd `U32.add_mod` xk `U32.add_mod` ti) <<< s)) in
   B.upd abcd a v;
+  
   let h' = HST.get () in
-  ()
-
-#reset-options
+  //reveal Spec.round_op_gen, also trigger sequence extensional equality rather than relying on z3
+  Spec.lemma_reveal_round_op_gen ();
+  assert (Seq.equal (B.as_seq h' abcd)
+                    (Spec.round_op_gen f (B.as_seq h abcd) (E.seq_uint32_of_le 16 (B.as_seq h x)) (U32.v a) (U32.v b) (U32.v c) (U32.v d) (U32.v k) s (U32.v i)))
+#pop-options
 
 inline_for_extraction let ia : abcd_idx = 0ul
 inline_for_extraction let ib : abcd_idx = 1ul
@@ -152,6 +159,8 @@ let round1
     B.as_seq h' abcd == Spec.round1 (B.as_seq h abcd) (E.seq_uint32_of_le 16 (B.as_seq h x))
   ))
 =
+  let h = HST.get () in
+
   let _ = round1_op abcd x ia ib ic id  0ul  7ul  1ul in
   let _ = round1_op abcd x id ia ib ic  1ul 12ul  2ul in
   let _ = round1_op abcd x ic id ia ib  2ul 17ul  3ul in
@@ -172,7 +181,9 @@ let round1
   let _ = round1_op abcd x ic id ia ib 14ul 17ul 15ul in
   let _ = round1_op abcd x ib ic id ia 15ul 22ul 16ul in
 
-  ()
+  let h' = HST.get () in
+  Spec.lemma_reveal_round1 ();
+  assert (Seq.equal (B.as_seq h' abcd) (Spec.round1 (B.as_seq h abcd) (E.seq_uint32_of_le 16 (B.as_seq h x))))
 
 inline_for_extraction
 let round2_op = round_op_gen Spec.g
@@ -194,6 +205,8 @@ let round2
     B.as_seq h' abcd == Spec.round2 (B.as_seq h abcd) (E.seq_uint32_of_le 16 (B.as_seq h x))
   ))
 =
+  let h = HST.get () in
+
   let _ = round2_op abcd x ia ib ic id 1ul 5ul 17ul in
   let _ = round2_op abcd x id ia ib ic 6ul 9ul 18ul in
   let _ = round2_op abcd x ic id ia ib 11ul 14ul 19ul in
@@ -214,7 +227,9 @@ let round2
   let _ = round2_op abcd x ic id ia ib 7ul 14ul 31ul in
   let _ = round2_op abcd x ib ic id ia 12ul 20ul 32ul in
 
-  ()
+  let h' = HST.get () in
+  Spec.lemma_reveal_round2 ();
+  assert (Seq.equal (B.as_seq h' abcd) (Spec.round2 (B.as_seq h abcd) (E.seq_uint32_of_le 16 (B.as_seq h x))))
 
 inline_for_extraction
 let round3_op = round_op_gen Spec.h
@@ -236,6 +251,8 @@ let round3
     B.as_seq h' abcd == Spec.round3 (B.as_seq h abcd) (E.seq_uint32_of_le 16 (B.as_seq h x))
   ))
 =
+  let h = HST.get () in
+
   let _ = round3_op abcd x ia ib ic id 5ul 4ul 33ul in
   let _ = round3_op abcd x id ia ib ic 8ul 11ul 34ul in
   let _ = round3_op abcd x ic id ia ib 11ul 16ul 35ul in
@@ -256,7 +273,9 @@ let round3
   let _ = round3_op abcd x ic id ia ib 15ul 16ul 47ul in
   let _ = round3_op abcd x ib ic id ia 2ul 23ul 48ul in
 
-  ()
+  let h' = HST.get () in
+  Spec.lemma_reveal_round3 ();
+  assert (Seq.equal (B.as_seq h' abcd) (Spec.round3 (B.as_seq h abcd) (E.seq_uint32_of_le 16 (B.as_seq h x))))
 
 inline_for_extraction
 let round4_op = round_op_gen Spec.i
@@ -278,6 +297,8 @@ let round4
     B.as_seq h' abcd == Spec.round4 (B.as_seq h abcd) (E.seq_uint32_of_le 16 (B.as_seq h x))
   ))
 =
+  let h = HST.get () in
+
   let _ = round4_op abcd x ia ib ic id 0ul 6ul 49ul in
   let _ = round4_op abcd x id ia ib ic 7ul 10ul 50ul in
   let _ = round4_op abcd x ic id ia ib 14ul 15ul 51ul in
@@ -298,7 +319,9 @@ let round4
   let _ = round4_op abcd x ic id ia ib 2ul 15ul 63ul in
   let _ = round4_op abcd x ib ic id ia 9ul 21ul 64ul in
 
-  ()
+  let h' = HST.get () in
+  Spec.lemma_reveal_round4 ();
+  assert (Seq.equal (B.as_seq h' abcd) (Spec.round4 (B.as_seq h abcd) (E.seq_uint32_of_le 16 (B.as_seq h x))))
 
 inline_for_extraction
 let rounds
@@ -317,11 +340,16 @@ let rounds
     B.as_seq h' abcd == Spec.rounds (B.as_seq h abcd) (E.seq_uint32_of_le 16 (B.as_seq h x))
   ))
 =
+  let h = HST.get () in
+
   round1 abcd x;
   round2 abcd x;
   round3 abcd x;
   round4 abcd x;
-  ()
+
+  let h' = HST.get () in
+  Spec.lemma_reveal_rounds ();
+  assert (Seq.equal (B.as_seq h' abcd) (Spec.rounds (B.as_seq h abcd) (E.seq_uint32_of_le 16 (B.as_seq h x))))
 
 inline_for_extraction
 let overwrite
@@ -335,12 +363,19 @@ let overwrite
       B.live h1 abcd /\
       B.as_seq h1 abcd == Spec.overwrite (B.as_seq h0 abcd) a' b' c' d'))
 = 
+  let h0 = HST.get () in
+
   B.upd abcd ia a';
   B.upd abcd ib b';
   B.upd abcd ic c';
-  B.upd abcd id d'
+  B.upd abcd id d';
 
-#reset-options "--z3rlimit 64 --z3cliopt smt.arith.nl=false --using_facts_from '* -FStar.Int8 -FStar.Int16 -FStar.Int32 -FStar.Int64 -FStar.Int128 -FStar.UInt16 -FStar.UInt64 -FStar.UInt128'"
+  let h1 = HST.get () in
+  Spec.lemma_reveal_overwrite ();
+  assert (Seq.equal (B.as_seq h1 abcd) (Spec.overwrite (B.as_seq h0 abcd) a' b' c' d'))
+
+(* No longer required *)
+//#reset-options "--z3rlimit 64 --z3cliopt smt.arith.nl=false --using_facts_from '* -FStar.Int8 -FStar.Int16 -FStar.Int32 -FStar.Int64 -FStar.Int128 -FStar.UInt16 -FStar.UInt64 -FStar.UInt128'"
 
 inline_for_extraction
 let update'
@@ -354,6 +389,8 @@ let update'
       B.live h1 abcd /\
       B.as_seq h1 abcd == Spec.update (B.as_seq h0 abcd) (B.as_seq h0 x)))
 =
+  let h0 = HST.get () in
+
   assert_norm (U32.v ia == Spec.ia);
   assert_norm (U32.v ib == Spec.ib);
   assert_norm (U32.v ic == Spec.ic);
@@ -371,15 +408,25 @@ let update'
     (a `U32.add_mod` aa)
     (b `U32.add_mod` bb)
     (c `U32.add_mod` cc)
-    (d `U32.add_mod` dd)
+    (d `U32.add_mod` dd);
 
-#reset-options
+  let h1 = HST.get () in
+  Spec.lemma_reveal_update ();
+  assert (Seq.equal (B.as_seq h1 abcd) (Spec.update (B.as_seq h0 abcd) (B.as_seq h0 x)))
 
+
+(* No longer required *)
+//#reset-options
+
+
+(*
+ * This squash proof is also no longer required, z3 can figure now
+ *)
 (* NOTE: do not remove this, and do not move this into the definition
    of `update` below: within `update` the context will be too crowded
    for F* to complete a proof of equality between two functions *)
-noextract
-let _ : squash (Spec.Hash.update MD5 == Spec.update) = ()
+//noextract
+//let _ : squash (Spec.Hash.update MD5 == Spec.update) = ()
 
 let update abcd x = update' abcd x
 
